Expand ra_mini and make dual test

crates/cachet-lang/src/type_checker.rs
@@ -1629,8 +1629,10 @@ fn is_const(expr: &Expr) -> bool {
         Expr::Negate(e) => is_const(&e.expr),
         Expr::Invoke(_)
         | Expr::FieldAccess(_)
-        | Expr::Cast(_)
         | Expr::Block(_)
         | Expr::Assign(_) => false,
+        Expr::Cast(cast_expr) => {
+            is_const(&cast_expr.expr) && matches!(cast_expr.type_, TypeIndex::BuiltIn(_))
+        }
     }
 }
