tests/dual/ra_mini.cpp
@@ -1,0 +1,54 @@
+#include <cassert>
+
+#define Cachet_Assert assert
+
+#include <cpp_prelude.h>
+#include <stdio.h>
+
+using namespace cachet::prelude;
+
+using Cachet_ContextRef = std::monostate;
+
+struct Range {
+    int32_t lower_;
+    int32_t upper_;
+    bool hasInt32LowerBound_;
+    bool hasInt32UpperBound_;
+    bool canHaveFractionalPart_;
+    bool canBeNegativeZero_;
+    uint16_t max_exponent_;
+};
+
+using JSVal = double;
+using Type_JSVal = PrimitiveType<JSVal*>;
+using Type_Range = PrimitiveType<Range*>;
+
+Type_Range::Val Fn_mk_range_raw(
+    std::monostate ctx,
+    int32_t lower_,
+    int32_t upper_,
+    bool hasInt32LowerBound_,
+    bool hasInt32UpperBound_,
+    bool canHaveFractionalPart_,
+    bool canBeNegativeZero_,
+    uint16_t max_exponent_
+) {
+    Range* r = new Range();
+    r->lower_ = lower_;
+    r->upper_ = upper_;
+    r->hasInt32LowerBound_ = hasInt32LowerBound_;
+    r->hasInt32UpperBound_ = hasInt32UpperBound_;
+    r->canBeNegativeZero_ = canBeNegativeZero_;
+    r->canHaveFractionalPart_ = canHaveFractionalPart_;
+    r->max_exponent_ = max_exponent_;
+    return r;
+}
+
+#include <test.h>
+#include <test.inc>
+
+int main() {
+    std::monostate ctx;
+    Fn_test(ctx);
+    return 0;
+}
